Iris/Iris/Algebra/BigOp.lean
@@ -892,7 +892,7 @@ open BigOpL MonoidOps
 @[rocq_alias big_opMS_empty, simp]
 theorem bigOpMS_empty {Φ : A → M} :
     ([^ op mset] x ∈ (∅ : MS), Φ x) = unit := by
-  show bigOpL op (fun _ x => Φ x) (FiniteMultiSet.toList (∅ : MS)) = unit
+  change bigOpL op (fun _ x => Φ x) (FiniteMultiSet.toList (∅ : MS)) = unit
   rw [LawfulFiniteMultiSet.toList_empty]; rfl
 
 @[rocq_alias big_opMS_elements]
@@ -901,7 +901,7 @@ theorem bigOpMS_bigOpL {Φ : A → M} {X : MS} :
 
 @[rocq_alias big_opMS_singleton]
 theorem bigOpMS_singleton {Φ : A → M} {a : A} : ([^ op mset] x ∈ ({a} : MS), Φ x) = Φ a := by
-  show bigOpL op (fun _ x => Φ x) (FiniteMultiSet.toList ({a} : MS)) = Φ a
+  change bigOpL op (fun _ x => Φ x) (FiniteMultiSet.toList ({a} : MS)) = Φ a
   rw [LawfulFiniteMultiSet.toList_singleton]
   exact bigOpL_singleton_eq (fun _ x => Φ x) a
 
