Iris/Iris/Algebra/Csum.lean
@@ -150,11 +150,11 @@ instance [OFE α] [OFE β] [IsCOFE α] [IsCOFE β] : IsCOFE (Csum α β) where
     revert h0n
     rcases e0 : c.chain 0 with a|b|_ <;> rcases en : c.chain n with a'|b'|_ <;> try (· exact id)
     · intro _
-      show IsCOFE.compl (chainL c a) ≡{n}≡ a'
+      change IsCOFE.compl (chainL c a) ≡{n}≡ a'
       refine OFE.Dist.trans COFE.conv_compl ?_
       simp [chainL, en]
     · intro _
-      show IsCOFE.compl (chainR c b) ≡{n}≡ b'
+      change IsCOFE.compl (chainR c b) ≡{n}≡ b'
       refine OFE.Dist.trans COFE.conv_compl ?_
       simp [chainR, en]
 
@@ -562,16 +562,16 @@ def cMap [CMRA α] [CMRA α'] [CMRA β] [CMRA β']
   pcore x := by
     cases x with
     | inl a =>
-      show ((CMRA.pcore a).map inl).map (map fa fb) = (CMRA.pcore (fa a)).map inl
+      change ((CMRA.pcore a).map inl).map (map fa fb) = (CMRA.pcore (fa a)).map inl
       rw [Option.map_map]
-      show (CMRA.pcore a).map (inl ∘ ⇑fa) = _
+      change (CMRA.pcore a).map (inl ∘ ⇑fa) = _
       rw [show (CMRA.pcore a).map (inl ∘ ⇑fa) = ((CMRA.pcore a).map fa).map inl from
         (Option.map_map ..).symm]
       exact Option.map_forall₂ inl (fa.pcore a)
     | inr b =>
-      show ((CMRA.pcore b).map inr).map (map fa fb) = (CMRA.pcore (fb b)).map inr
+      change ((CMRA.pcore b).map inr).map (map fa fb) = (CMRA.pcore (fb b)).map inr
       rw [Option.map_map]
-      show (CMRA.pcore b).map (inr ∘ ⇑fb) = _
+      change (CMRA.pcore b).map (inr ∘ ⇑fb) = _
       rw [show (CMRA.pcore b).map (inr ∘ ⇑fb) = ((CMRA.pcore b).map fb).map inr from
         (Option.map_map ..).symm]
       exact Option.map_forall₂ inr (fb.pcore b)
