Iris/Iris/Algebra/HeapView.lean
@@ -702,7 +702,7 @@ theorem update_big_replace (m m0 m1 : H V)
       · simpa [dom, get?_delete_ne hjk, get?_insert_ne hjk] using congrFun Hdom j
     have hunion : (m1 ∪ m) = Std.insert (delete m1 k ∪ m) k v' :=
       eqv_of_Equiv fun j => by
-        show get? (PartialMap.union m1 m) j
+        change get? (PartialMap.union m1 m) j
           = get? (Std.insert (PartialMap.union (delete m1 k) m) k v') j
         by_cases hjk : k = j
         · rw [← hjk, get?_insert_eq rfl]
