Iris/Iris/BI/Embedding.lean
@@ -448,7 +448,7 @@ theorem embed_internal_eq {A : Type _} [OFE A] (x y : A) :
 
 @[rocq_alias embed_plainly]
 theorem embed_plainly (P : P1) : (⎡■ P⎤ : P2) ⊣⊢ ■ ⎡P⎤ := by
-  show (embed (SiPure.siPure (SiEmpValid.siEmpValid P)) : P2)
+  change (embed (SiPure.siPure (SiEmpValid.siEmpValid P)) : P2)
       ⊣⊢ SiPure.siPure (SiEmpValid.siEmpValid (embed P))
   exact (embed_siPure _).trans
     ⟨siPure_mono (BiEmbedSbi.embed_siEmpValid P).mpr,
